state of the bug

code/curve25519/Hacl.Meta.Curve25519.fst
@@ -3,9 +3,253 @@ module Hacl.Meta.Curve25519
 #set-options "--max_fuel 2 --max_ifuel 1 --z3rlimit 300 --print_implicits --print_full_names"
 
 // For debugging
-#set-options "--admit_smt_queries true"
+#set-options "--admit_smt_queries true --print_effect_args"
 
 friend Hacl.Impl.Curve25519.Generic
+
+// START DEBUGGING
+
+let ( |+| ) = Lib.Buffer.(( |+| ))
+open FStar.Mul
+
+%splice[
+  carry_pass_store_higher
+]
+(Meta.Interface.specialize (`Hacl.Impl.Curve25519.Fields.field_spec) [
+  `Hacl.Impl.Curve25519.Field64.carry_pass_store
+])
+
+let store_felem_higher_t: Type0 = 
+    u64s28607: Lib.Buffer.lbuffer Lib.IntTypes.uint64 4ul ->
+    f28608: Hacl.Impl.Curve25519.Field64.felem
+  -> FStar.HyperStack.ST.Stack Prims.unit
+      (fun h28609 ->
+          Prims.b2t Vale.X64.CPU_Features_s.adx_enabled /\
+          Prims.b2t Vale.X64.CPU_Features_s.bmi2_enabled /\
+          Lib.Buffer.live #(Lib.Buffer.MUT) #Lib.IntTypes.uint64 h28609 f28608 /\
+          Lib.Buffer.live #(Lib.Buffer.MUT) #Lib.IntTypes.uint64 h28609 u64s28607 /\
+          Lib.Buffer.disjoint #(Lib.Buffer.MUT)
+            #(Lib.Buffer.MUT)
+            #Lib.IntTypes.uint64
+            #Lib.IntTypes.uint64
+            u64s28607
+            f28608)
+      (fun h028610 _ h128612 ->
+          Lib.Buffer.modifies (Lib.Buffer.loc #(Lib.Buffer.MUT) #Lib.IntTypes.uint64 u64s28607 |+|
+              Lib.Buffer.loc #(Lib.Buffer.MUT) #Lib.IntTypes.uint64 f28608)
+            h028610
+            h128612 /\
+          Prims.eq2 #(s28613:
+              Lib.Sequence.seq Lib.IntTypes.uint64
+                { Prims.eq2 #Prims.nat
+                    (FStar.Seq.Base.length #Lib.IntTypes.uint64 s28613)
+                    (Lib.IntTypes.v #(Lib.IntTypes.U32)
+                        #(Lib.IntTypes.PUB)
+                        4ul) \/
+                  Prims.eq2 #Prims.nat
+                    (Lib.Sequence.length #(Lib.IntTypes.uint_t (Lib.IntTypes.U64) (Lib.IntTypes.SEC)
+                        )
+                        s28613)
+                    4 /\
+                  Prims.eq2 #(n28614:
+                      Prims.nat
+                        { Prims.b2t (n28614 <
+                              Prims.pow2 (Lib.Sequence.length #(Lib.IntTypes.uint_t (Lib.IntTypes.U64
+                                        )
+                                        (Lib.IntTypes.SEC))
+                                    s28613 *
+                                  Lib.IntTypes.bits (Lib.IntTypes.U64))) \/
+                          Prims.b2t (n28614 < Prims.pow2 (Lib.IntTypes.bits (Lib.IntTypes.U64) * 4))
+                        })
+                    (Hacl.Impl.Curve25519.Field64.Core.fevalh h028610 f28608)
+                    (Lib.ByteSequence.nat_from_intseq_le #(Lib.IntTypes.U64)
+                        #(Lib.IntTypes.SEC)
+                        s28613) })
+            (Lib.Buffer.as_seq #(Lib.Buffer.MUT)
+                #Lib.IntTypes.uint64
+                #4ul
+                h128612
+                u64s28607)
+            (Lib.ByteSequence.nat_to_intseq_le #(Lib.IntTypes.U64)
+                #(Lib.IntTypes.SEC)
+                4
+                (Hacl.Impl.Curve25519.Field64.Core.fevalh h028610 f28608)))
+
+let store_felem_higher:
+
+    arg_Hacl_Impl_Curve25519_Field64_Core_add128696:
+      (
+            out28697: Hacl.Impl.Curve25519.Field64.Core.u256 ->
+            f128698: Hacl.Impl.Curve25519.Field64.Core.u256 ->
+            f228699: Lib.IntTypes.uint64
+          -> FStar.HyperStack.ST.Stack Lib.IntTypes.uint64
+              (fun h28700 ->
+                  Prims.b2t Vale.X64.CPU_Features_s.adx_enabled /\
+                  Prims.b2t Vale.X64.CPU_Features_s.bmi2_enabled /\
+                  Lib.Buffer.live #(Lib.Buffer.MUT) #Lib.IntTypes.uint64 h28700 f128698 /\
+                  Lib.Buffer.live #(Lib.Buffer.MUT) #Lib.IntTypes.uint64 h28700 out28697 /\
+                  (Lib.Buffer.disjoint #(Lib.Buffer.MUT)
+                      #(Lib.Buffer.MUT)
+                      #Lib.IntTypes.uint64
+                      #Lib.IntTypes.uint64
+                      out28697
+                      f128698 \/ Prims.eq2 #Hacl.Impl.Curve25519.Field64.Core.u256 out28697 f128698)
+              )
+              (fun h028701 c28702 h128703 ->
+                  Lib.Buffer.modifies (Lib.Buffer.loc #(Lib.Buffer.MUT)
+                        #Lib.IntTypes.uint64
+                        out28697)
+                    h028701
+                    h128703 /\
+                  Prims.eq2 #Prims.int
+                    (Hacl.Impl.Curve25519.Field64.Core.as_nat h128703 out28697 +
+                      Lib.IntTypes.v #(Lib.IntTypes.U64) #(Lib.IntTypes.SEC) c28702 * Prims.pow2 256
+                    )
+                    (Hacl.Impl.Curve25519.Field64.Core.as_nat h028701 f128698 +
+                      Lib.IntTypes.v #(Lib.IntTypes.U64) #(Lib.IntTypes.SEC) f228699)))
+  -> Prims.Tot store_felem_higher_t
+=
+fun arg_Hacl_Impl_Curve25519_Field64_Core_add128704 u64s28705 f28706 ->
+  let h028707 = FStar.HyperStack.ST.get () in
+  let _uu___28708 =
+    carry_pass_store_higher arg_Hacl_Impl_Curve25519_Field64_Core_add128704
+      f28706
+  in
+  let h128709 = FStar.HyperStack.ST.get () in
+  let _uu___28710 =
+    Hacl.Spec.Curve25519.Field64.lemma_carry_pass_store0 (Hacl.Impl.Curve25519.Field64.as_tup4 h028707
+          f28706)
+  in
+  let _uu___28711 =
+    carry_pass_store_higher arg_Hacl_Impl_Curve25519_Field64_Core_add128704
+      f28706
+  in
+  let h228712 = FStar.HyperStack.ST.get () in
+  let _uu___28713 =
+    Hacl.Spec.Curve25519.Field64.lemma_carry_pass_store1 (Hacl.Impl.Curve25519.Field64.as_tup4 h128709
+          f28706)
+  in
+  let f028714 =
+    Lib.Buffer.op_Array_Access #(Lib.Buffer.MUT)
+      #Lib.IntTypes.uint64
+      #4ul
+      f28706
+      0ul
+  in
+  let f128715 =
+    Lib.Buffer.op_Array_Access #(Lib.Buffer.MUT)
+      #Lib.IntTypes.uint64
+      #4ul
+      f28706
+      1ul
+  in
+  let f228716 =
+    Lib.Buffer.op_Array_Access #(Lib.Buffer.MUT)
+      #Lib.IntTypes.uint64
+      #4ul
+      f28706
+      2ul
+  in
+  let f328717 =
+    Lib.Buffer.op_Array_Access #(Lib.Buffer.MUT)
+      #Lib.IntTypes.uint64
+      #4ul
+      f28706
+      3ul
+  in
+  let _uu___28718 =
+    assert (Prims.b2t (Prims.op_LessThan (Lib.IntTypes.v #(Lib.IntTypes.U64)
+                  #(Lib.IntTypes.SEC)
+                  f328717)
+              (Prims.pow2 63)))
+  in
+  let _uu___28719 =
+    assert (Prims.b2t (Prims.op_LessThan (Hacl.Impl.Curve25519.Field64.Core.as_nat h228712 f28706)
+              (Prims.pow2 255)))
+  in
+  let _uu___28720 =
+    Hacl.Spec.Curve25519.Field64.subtract_p4 (FStar.Pervasives.Native.Mktuple4 #Lib.IntTypes.uint64
+          #Lib.IntTypes.uint64
+          #Lib.IntTypes.uint64
+          #Lib.IntTypes.uint64
+          f028714
+          f128715
+          f228716
+          f328717)
+  in
+  let FStar.Pervasives.Native.Mktuple4 #_ #_ #_ #_ o028721 o128722 o228723 o328724 = _uu___28720 in
+  let _uu___28725 =
+    assert (Prims.b2t (Prims.op_LessThan (Hacl.Spec.Curve25519.Field64.Definition.as_nat4 (FStar.Pervasives.Native.Mktuple4
+                      #Lib.IntTypes.uint64
+                      #Lib.IntTypes.uint64
+                      #Lib.IntTypes.uint64
+                      #Lib.IntTypes.uint64
+                      o028721
+                      o128722
+                      o228723
+                      o328724))
+              Spec.Curve25519.prime))
+  in
+  let _uu___28726 =
+    assert (Prims.eq2 #Prims.int
+          (Hacl.Spec.Curve25519.Field64.Definition.as_nat4 (FStar.Pervasives.Native.Mktuple4
+                  #Lib.IntTypes.uint64
+                  #Lib.IntTypes.uint64
+                  #Lib.IntTypes.uint64
+                  #Lib.IntTypes.uint64
+                  o028721
+                  o128722
+                  o228723
+                  o328724))
+          (Prims.op_Modulus (Hacl.Impl.Curve25519.Field64.Core.as_nat h228712 f28706)
+              Spec.Curve25519.prime))
+  in
+  let _uu___28727 =
+    Lib.Buffer.op_Array_Assignment #Lib.IntTypes.uint64
+      #4ul
+      u64s28705
+      0ul
+      o028721
+  in
+  let _uu___28728 =
+    Lib.Buffer.op_Array_Assignment #Lib.IntTypes.uint64
+      #4ul
+      u64s28705
+      1ul
+      o128722
+  in
+  let _uu___28729 =
+    Lib.Buffer.op_Array_Assignment #Lib.IntTypes.uint64
+      #4ul
+      u64s28705
+      2ul
+      o228723
+  in
+  let _uu___28730 =
+    Lib.Buffer.op_Array_Assignment #Lib.IntTypes.uint64
+      #4ul
+      u64s28705
+      3ul
+      o328724
+  in
+  let h328731 = FStar.HyperStack.ST.get () in
+  let _uu___28732 =
+    Hacl.Impl.Curve25519.Lemmas.lemma_nat_from_uints64_le_4 (Lib.Buffer.as_seq #(Lib.Buffer.MUT)
+          #Lib.IntTypes.uint64
+          #4ul
+          h328731
+          u64s28705)
+  in
+  Lib.ByteSequence.lemma_nat_from_to_intseq_le_preserves_value #(Lib.IntTypes.U64)
+    #(Lib.IntTypes.SEC)
+    4
+    (Lib.Buffer.as_seq #(Lib.Buffer.MUT)
+        #Lib.IntTypes.uint64
+        #4ul
+        h328731
+        u64s28705)
+
+// END DEBUGGING
 
 %splice[
 (*  // From Finv.
